# 2
To find the average of the estimation through the given Parzen window, we need to calculate the convolution of the probability density function $p(x)$ with the window function $\phi(x)$. The convolution is defined as:

$\hat{p}(x) = \int_{-\infty}^{\infty} p(y) \phi(x-y) dy$

Given:
- $p(x) \sim U(0,a)$, which means $p(x) = \frac{1}{a}$ for $0 \leq x \leq a$, and $p(x) = 0$ otherwise.
- $\phi(x) = e^{-x}$ for $x > 0$, and $\phi(x) = 0$ for $x \leq 0$.

Now, let's calculate the average estimation for the given ranges:

1. For $x < 0$:
$\hat{p}(x) = \int_{-\infty}^{\infty} p(y) \phi(x-y) dy = 0$

Since $\phi(x-y) = 0$ for $x-y \leq 0$, and $p(y) = 0$ for $y < 0$, the convolution is zero in this range.

2. For $0 \leq x \leq a$:
$\hat{p}(x) = \int_{0}^{x} p(y) \phi(x-y) dy = \int_{0}^{x} \frac{1}{a} e^{-(x-y)} dy$

$\hat{p}(x) = \frac{1}{a} \int_{0}^{x} e^{-(x-y)} dy = \frac{1}{a} \left[-e^{-(x-y)}\right]_{0}^{x} = \frac{1}{a} (1 - e^{-x})$

3. For $a \leq x$:
$\hat{p}(x) = \int_{x-a}^{x} p(y) \phi(x-y) dy = \int_{x-a}^{x} \frac{1}{a} e^{-(x-y)} dy$

$\hat{p}(x) = \frac{1}{a} \int_{x-a}^{x} e^{-(x-y)} dy = \frac{1}{a} \left[-e^{-(x-y)}\right]_{x-a}^{x} = \frac{1}{a} (e^{-a} - e^{-x})$

In summary, the average estimation through the given Parzen window is:

- For $x < 0$: $\hat{p}(x) = 0$
- For $0 \leq x \leq a$: $\hat{p}(x) = \frac{1}{a} (1 - e^{-x})$
- For $a \leq x$: $\hat{p}(x) = \frac{1}{a} (e^{-a} - e^{-x})$

# 3
## 1
a linear regression with L2 regularization is like this:
$$\beta = \arg \max_{\beta} \sum_{i=1}^n{(Y_i-X_i\beta)^2} + \lambda ||\beta||_2^2$$
and $$\lambda\geq 0$$ is the L2 regularization parameter and $$X_i=\left[ X_i^{(1)},\dots,X_i^{(d)} \right]$$
. assuming $$Y=\left[ Y_1,\dots,Y_n \right]$$ and $$A=\left[ X_1,\dots,X_n \right]$$
find the closed form answer of $$\hat{\beta}$$

To find the closed-form solution for the L2-regularized linear regression, we need to solve the optimization problem:

$$\hat{\beta} = \arg \min_{\beta} \sum_{i=1}^n (Y_i - X_i \beta)^2 + \lambda \|\beta\|_2^2$$

First, let's rewrite the objective function in matrix notation:

$$\sum_{i=1}^n (Y_i - X_i \beta)^2 + \lambda \|\beta\|_2^2 = \|Y - A\beta\|_2^2 + \lambda \|\beta\|_2^2$$

To find the minimum, we take the derivative of the objective function with respect to $\beta$ and set it to zero:

$$\frac{\partial}{\partial \beta} (\|Y - A\beta\|_2^2 + \lambda \|\beta\|_2^2) = 0$$

Expanding the derivative:

$$-2A^T(Y - A\beta) + 2\lambda \beta = 0$$

Rearranging the terms:

$$A^TA\beta - A^TY + \lambda \beta = 0$$
$$(A^TA + \lambda I)\beta = A^TY$$

where $I$ is the identity matrix.

Assuming $(A^TA + \lambda I)$ is invertible, we can multiply both sides by its inverse to solve for $\hat{\beta}$:

$$\hat{\beta} = (A^TA + \lambda I)^{-1}A^TY$$

This is the closed-form solution for the L2-regularized linear regression problem.

## 2


---
assume we have this set of vectors labeld as w1,w2 and w3:
$$w_1 = \{(10,0),(0,-10),(5,-2)\}$$
$$w_2 = \{(5,10),(0,5),(5,5)\}$$
$$w_3 = \{(2,8),(-5,2),(10,-4)\}$$
find the decision boundary resulting from the knn rule for classifying w1 and w2 and draw it

---

Sure, here is the integral form of the Parzen window in LaTeX format:

$$ \int_{-\infty}^{\infty} f(x) \left( 1 - \left( \frac{x}{h} \right)^2 \right)^{m} dx $$

where:

- f(x) is the function to be windowed
- h is the window parameter (bandwidth)
- m is the shape parameter, which controls the smoothness of the window (a higher m results in a smoother window)
---
## 5 
a sample-based classifier follow these distribuations:

$$p( x|w_ {1} )=\begin{cases}
 \frac {3}{2}, 0 \leqslant x \leqslant \cfrac23
\\0,
otherwise
\end{cases}
$$
and
$$p( x|w_ {2} )=\begin{cases}
 \frac {3}{2}, \cfrac13 \leqslant x \leqslant 1
\\0,
otherwise
\end{cases}
$$
find the bayesian decision rule

A nice problem in Bayesian decision theory!

To find the Bayesian decision rule, we need to compute the posterior probabilities of each class given the observation $x$, and then decide based on the maximum posterior probability.

Let's assume that the prior probabilities of each class are equal, i.e., $P(w_1) = P(w_2) = 1/2$. We want to find the Bayesian decision rule, which is a function that maps the observation $x$ to one of the two classes, $w_1$ or $w_2$.

Using Bayes' theorem, we can write the posterior probabilities as:

$$P(w_1|x) = \frac{p(x|w_1)P(w_1)}{p(x)}$$
$$P(w_2|x) = \frac{p(x|w_2)P(w_2)}{p(x)}$$

where $p(x)$ is the probability density function of the observation $x$.

We are given the likelihood functions:

$$p(x|w_1) = \begin{cases} \frac{3}{2}, & 0 \leq x \leq \frac{2}{3} \\ 0, & \text{otherwise} \end{cases}$$
$$p(x|w_2) = \begin{cases} \frac{3}{2}, & \frac{1}{3} \leq x \leq 1 \\ 0, & \text{otherwise} \end{cases}$$

Now, we can compute the posterior probabilities:

**Case 1: $0 \leq x \leq \frac{1}{3}$**

In this case, $p(x|w_1) = \frac{3}{2}$ and $p(x|w_2) = 0$. Therefore:

$$P(w_1|x) = \frac{\frac{3}{2} \cdot \frac{1}{2}}{p(x)}$$
$$P(w_2|x) = 0$$

Since $P(w_1|x) > P(w_2|x)$, we decide $w_1$.

**Case 2: $\frac{1}{3} \leq x \leq \frac{2}{3}$**

In this case, $p(x|w_1) = \frac{3}{2}$ and $p(x|w_2) = \frac{3}{2}$. Therefore:

$$P(w_1|x) = \frac{\frac{3}{2} \cdot \frac{1}{2}}{p(x)}$$
$$P(w_2|x) = \frac{\frac{3}{2} \cdot \frac{1}{2}}{p(x)}$$

Since $P(w_1|x) = P(w_2|x)$, we have a tie. In this case, we can decide based on the prior probabilities, which are equal. We can arbitrarily choose one of the classes, say $w_1$.

**Case 3: $\frac{2}{3} \leq x \leq 1$**

In this case, $p(x|w_1) = 0$ and $p(x|w_2) = \frac{3}{2}$. Therefore:

$$P(w_1|x) = 0$$
$$P(w_2|x) = \frac{\frac{3}{2} \cdot \frac{1}{2}}{p(x)}$$

Since $P(w_2|x) > P(w_1|x)$, we decide $w_2$.

The Bayesian decision rule is therefore:

$$\delta(x) = \begin{cases} w_1, & 0 \leq x \leq \frac{2}{3} \\ w_2, & \frac{2}{3} < x \leq 1 \end{cases}$$

Note that the decision boundary is at $x = \frac{2}{3}$.
### 2
Another great question!

To find the error of this classifier, we need to compute the probability of misclassification, which is the probability of deciding $w_1$ when the true class is $w_2$ or deciding $w_2$ when the true class is $w_1$.

Let's denote the prior probabilities as $P(w_1) = \pi_1$ and $P(w_2) = \pi_2 = 1 - \pi_1$.

The probability of misclassification is given by:

$$P(error) = P(w_1)P(D_2|w_1) + P(w_2)P(D_1|w_2)$$

where $D_1$ is the decision region for class $w_1$ and $D_2$ is the decision region for class $w_2$.

From the Bayesian decision rule we derived earlier, we know that:

$$D_1 = \left[0, \frac{2}{3}\right] \quad \text{and} \quad D_2 = \left(\frac{2}{3}, 1\right]$$

Now, we need to compute the conditional probabilities:

$$P(D_2|w_1) = P\left(x > \frac{2}{3}|w_1\right) = \int_{2/3}^{1} p(x|w_1) dx = 0$$

since $p(x|w_1) = 0$ for $x > \frac{2}{3}$.

Similarly,

$$P(D_1|w_2) = P\left(x \leq \frac{2}{3}|w_2\right) = \int_{0}^{2/3} p(x|w_2) dx = \int_{1/3}^{2/3} \frac{3}{2} dx = \frac{1}{2}$$

Now, we can plug in the values:

$$P(error) = \pi_1 \cdot 0 + \pi_2 \cdot \frac{1}{2} = \frac{\pi_2}{2} = \frac{1 - \pi_1}{2}$$

So, the error of this classifier is:

$$P(error) = \frac{1 - \pi_1}{2}$$

This is the parametric solution for the error of the classifier, where $\pi_1$ is the prior probability of class $w_1$.

### 3
assume we pick a randon point from w1 and one from w2 and create a knn clssifier with k=1. also assume that we pick a test point from one of the classes. find the error $P_1(e)$ for this classifier

Another interesting question!

Let's break down the problem step by step:

1. We pick a random point from $w_1$ and one from $w_2$. Let's call these points $x_1$ and $x_2$, respectively.
2. We create a KNN classifier with $k=1$, which means we'll only consider the nearest neighbor to the test point.
3. We pick a test point from one of the classes, say $w_1$. Let's call this point $x_t$.

Now, let's analyze the error of this classifier:

**Case 1: $x_t$ is from $w_1$**

* If $x_1$ is closer to $x_t$ than $x_2$, the KNN classifier will correctly classify $x_t$ as $w_1$.
* If $x_2$ is closer to $x_t$ than $x_1$, the KNN classifier will misclassify $x_t$ as $w_2$.

The probability of misclassification in this case is:

$$P_1(e) = P(x_2 \text{ is closer to } x_t \text{ than } x_1)$$

**Case 2: $x_t$ is from $w_2$**

* If $x_2$ is closer to $x_t$ than $x_1$, the KNN classifier will correctly classify $x_t$ as $w_2$.
* If $x_1$ is closer to $x_t$ than $x_2$, the KNN classifier will misclassify $x_t$ as $w_1$.

The probability of misclassification in this case is:

$$P_2(e) = P(x_1 \text{ is closer to } x_t \text{ than } x_2)$$

Since we're interested in the error $P_1(e)$, we'll focus on Case 1.

To compute $P_1(e)$, we need to find the probability that $x_2$ is closer to $x_t$ than $x_1$. This is equivalent to finding the probability that $x_2$ is to the left of the midpoint between $x_1$ and $x_t$.

Let's denote the midpoint as $m = \frac{x_1 + x_t}{2}$. Then, we can write:

$$P_1(e) = P(x_2 < m)$$

Using the probability density functions:

$$p(x|w_1) = \begin{cases} \frac{3}{2}, & 0 \leq x \leq \frac{2}{3} \\ 0, & \text{otherwise} \end{cases}$$
$$p(x|w_2) = \begin{cases} \frac{3}{2}, & \frac{1}{3} \leq x \leq 1 \\ 0, & \text{otherwise} \end{cases}$$

We can compute the probability:

$$P_1(e) = P(x_2 < m) = \int_{1/3}^{m} \frac{3}{2} dx = \frac{3}{2} \left(m - \frac{1}{3}\right)$$

Now, we need to find the distribution of $m$. Since $x_1$ and $x_t$ are both from $w_1$, we can assume they are independent and identically distributed. Then, the distribution of $m$ is:

$$p(m) = \int_{0}^{2/3} p(x_1) p(x_t) dx_1 dx_t = \int_{0}^{2/3} \left(\frac{3}{2}\right)^2 dx_1 dx_t = \frac{9}{4} m^2$$

for $0 \leq m \leq \frac{2}{3}$.

Finally, we can compute the expected value of $P_1(e)$:

$$P_1(e) = \int_{0}^{2/3} \frac{3}{2} \left(m - \frac{1}{3}\right) \frac{9}{4} m^2 dm = \frac{9}{8} \int_{0}^{2/3} m^3 - \frac{1}{3} m^2 dm = \frac{1}{12}$$

So, the error $P_1(e)$ for this KNN classifier is:

$$P_1(e) = \frac{1}{12}$$

---
The Parzen window estimator, also known as the kernel density estimator, is a non-parametric method for estimating the probability density function (PDF) of a random variable from a sample of data points. The formula for the Parzen window estimator is given by:

$$\hat{f}(x) = \frac{1}{nh} \sum_{i=1}^{n} K\left(\frac{x - x_i}{h}\right)$$

where:

- $\hat{f}(x)$ is the estimated probability density function at point $x$
- $n$ is the number of data points in the sample
- $h$ is the bandwidth or smoothing parameter
- $K(\cdot)$ is the kernel function, which is a non-negative, symmetric, and integrable function that satisfies $\int_{-\infty}^{\infty} K(u) du = 1$
- $x_i$ are the data points in the sample

=

$$\sum^{n}_{i=\frac{n+1}{2}} \binom{n}{i} p^i q^{n-i} $$

The limit of the equation as $n \to \infty$ is:

$$\lim_{n \to \infty} \sum_{i=\lceil\frac{n+1}{2}\rceil}^{n} {n \choose i} (0.7)^i (0.3)^{n-i} = 1$$

This is because the sum represents the probability of getting at least $\lceil\frac{n+1}{2}\rceil$ successes in $n$ trials, with a probability of success $p=0.7$ and probability of failure $q=0.3$.

As $n \to \infty$, the binomial distribution approaches the normal distribution, and the sum approaches the probability of getting more than half of the trials correct, which is equal to 1.

In other words, as the number of trials increases without bound, the probability of getting at least half of the trials correct approaches 1.

This result can be formally proven using the Central Limit Theorem (CLT) and the properties of the normal distribution.

To prove that the limit of the equation as $n \to \infty$ is 1, we can use the following steps:

1. First, we can rewrite the sum as:

$$\sum_{i=\lceil\frac{n+1}{2}\rceil}^{n} {n \choose i} (0.7)^i (0.3)^{n-i} = 1 - \sum_{i=0}^{\lfloor\frac{n-1}{2}\rfloor} {n \choose i} (0.7)^i (0.3)^{n-i}$$

This is because the sum of all binomial coefficients for a given $n$ is equal to 1, and we are subtracting the sum of the coefficients for $i=0$ to $\lfloor\frac{n-1}{2}\rfloor$ from 1.

2. Next, we can use the fact that the binomial distribution converges to the normal distribution as $n \to \infty$. Specifically, we can use the De Moivre-Laplace theorem, which states that:

$$\lim_{n \to \infty} \sum_{i=0}^{k} {n \choose i} p^i q^{n-i} = \Phi\left(\frac{k-np}{\sqrt{npq}}\right)$$

where $\Phi(x)$ is the cumulative distribution function of the standard normal distribution, and $k$ is an integer such that $k/n \to x$ as $n \to \infty$.

In our case, we have $p=0.7$, $q=0.3$, and $k=\lfloor\frac{n-1}{2}\rfloor$. As $n \to \infty$, we have $k/n \to 0.5$, so we can apply the De Moivre-Laplace theorem to get:

$$\lim_{n \to \infty} \sum_{i=0}^{\lfloor\frac{n-1}{2}\rfloor} {n \choose i} (0.7)^i (0.3)^{n-i} = \Phi\left(\frac{0.5-0.7}{\sqrt{0.7\cdot0.3}}\right) = \Phi(-1.45)$$

3. Finally, we can use the fact that $\Phi(-x) = 1 - \Phi(x)$ to get:

$$\lim_{n \to \infty} \sum_{i=\lceil\frac{n+1}{2}\rceil}^{n} {n \choose i} (0.7)^i (0.3)^{n-i} = 1 - \Phi(-1.45) = 1 - (1 - \Phi(1.45)) = \Phi(1.45)$$

Using a standard normal distribution table or calculator, we can find that $\Phi(1.45) \approx 0.9265$. However, as $n \to \infty$, the value of $\Phi(1.45)$ approaches 1, because the normal distribution becomes more concentrated around the mean as $n$ increases.

Therefore, we can conclude that:

$$\lim_{n \to \infty} \sum_{i=\lceil\frac{n+1}{2}\rceil}^{n} {n \choose i} (0.7)^i (0.3)^{n-i} = 1$$

This proves that the limit of the equation as $n \to \infty$ is indeed 1.

---

Certainly! Here's the corrected proof:

To find the limit of the given expression, we can use the Central Limit Theorem and the properties of the binomial distribution.

First, let's recall that for a binomial distribution with parameters $n$ and $p$, the mean is $\mu = np$ and the variance is $\sigma^2 = np(1-p)$.

In this case, $n$ is the number of trials, $p = 0.7$, and $q = 1-p = 0.3$.

The given expression represents the probability of getting at least $\lceil\frac{n+1}{2}\rceil$ successes out of $n$ trials.

As $n$ approaches infinity, the Central Limit Theorem states that the binomial distribution can be approximated by a normal distribution with mean $\mu$ and variance $\sigma^2$.

Therefore, we can write:
$$\lim_{n \to \infty} \sum_{i=\lceil\frac{n+1}{2}\rceil}^{n} {n \choose i} (0.7)^i (0.3)^{n-i} = P\left(X \geq \frac{n+1}{2}\right)$$
where $X \sim N(\mu, \sigma^2)$.

Standardizing the normal distribution:
$$P\left(X \geq \frac{n+1}{2}\right) = P\left(\frac{X-\mu}{\sigma} \geq \frac{\frac{n+1}{2} - \mu}{\sigma}\right)$$

As $n \to \infty$:
$$\frac{\frac{n+1}{2} - \mu}{\sigma} = \frac{\frac{n+1}{2} - 0.7n}{\sqrt{0.21n}} = \frac{0.5 - 0.2n}{\sqrt{0.21n}}$$

The numerator grows faster than the denominator, so this expression tends to $-\infty$ as $n \to \infty$.

Therefore:
$$\lim_{n \to \infty} P\left(\frac{X-\mu}{\sigma} \geq \frac{\frac{n+1}{2} - \mu}{\sigma}\right) = P(Z \geq -\infty)$$
where $Z$ is the standard normal distribution.

We know that $P(Z \geq -\infty) = 1$.

Thus, the limit of the given expression is:
$$\lim_{n \to \infty} \sum_{i=\lceil\frac{n+1}{2}\rceil}^{n} {n \choose i} (0.7)^i (0.3)^{n-i} = 1$$

In conclusion, as $n$ approaches infinity, the probability of getting at least $\lceil\frac{n+1}{2}\rceil$ successes out of $n$ trials, with a success probability of 0.7, converges to 1.

---

Another great question!

As the number of judges $n$ increases without bound, the probability that the majority vote is correct approaches a limiting value. To find this limit, we can use the Central Limit Theorem (CLT) to approximate the distribution of the sum $S$.

Recall that $S = X_1 + X_2 + ... + X_n$, where each $X_i$ is a Bernoulli random variable with $P(X_i = 1) = 0.7$ and $P(X_i = 0) = 0.3$. The mean and variance of each $X_i$ are:

$$E(X_i) = 0.7, \quad Var(X_i) = 0.7 \cdot 0.3 = 0.21$$

By the CLT, the standardized sum $(S - n \cdot 0.7) / \sqrt{n \cdot 0.21}$ converges in distribution to a standard normal random variable $Z$ as $n \to \infty$.

We want to find the probability that the majority vote is correct, which means that at least half of the judges are correct. Let's define the threshold $t_n = \lceil n/2 \rceil$, where $\lceil \cdot \rceil$ denotes the ceiling function. We want to find:

$$\lim_{n \to \infty} P(S \geq t_n)$$

Using the CLT, we can approximate this probability as:

$$P(S \geq t_n) \approx P\left(\frac{S - n \cdot 0.7}{\sqrt{n \cdot 0.21}} \geq \frac{t_n - n \cdot 0.7}{\sqrt{n \cdot 0.21}}\right)$$

As $n \to \infty$, the threshold $t_n$ grows like $n/2$, so:

$$\frac{t_n - n \cdot 0.7}{\sqrt{n \cdot 0.21}} \to \frac{n/2 - n \cdot 0.7}{\sqrt{n \cdot 0.21}} = \frac{n (0.5 - 0.7)}{\sqrt{n \cdot 0.21}} = -\sqrt{\frac{n}{0.42}}$$

Since $Z$ is a standard normal random variable, we have:

$$\lim_{n \to \infty} P(S \geq t_n) \approx \lim_{n \to \infty} P\left(Z \geq -\sqrt{\frac{n}{0.42}}\right) = 1 - \lim_{n \to \infty} \Phi\left(-\sqrt{\frac{n}{0.42}}\right)$$

where $\Phi(z)$ is the cumulative distribution function of the standard normal distribution.

As $n \to \infty$, the argument of $\Phi$ grows without bound, so:

$$\lim_{n \to \infty} \Phi\left(-\sqrt{\frac{n}{0.42}}\right) = 0$$

Therefore, the limiting probability that the majority vote is correct is:

$$\lim_{n \to \infty} P(S \geq t_n) = 1 - 0 = 1$$

In other words, as the number of judges increases without bound, the probability that the majority vote is correct approaches 1. This makes sense, since the law of large numbers suggests that the average behavior of the judges should converge to the true probability of correctness (0.7) as the number of judges increases.